examples/Bisimilarity/CADP/Size1/Terms.v
@@ -6,12 +6,12 @@ From Stdlib Require Import Relations.Relation_Operators.
 From Stdlib Require Operators_Properties.
 
 Require Import MEBI.Examples.CADP.
-Import Protocol. 
 
 Require Import MEBI.Examples.CADP_Glued.
 
 MeBi Divider "Examples.Bisimilarity.CADP.Size1.Terms".
 
-Example p1 : tm * env := (P, Env.initial 1).
+Example p1 : process := process_create 0 Protocol.P.
 
-Example c1 : composition := compose (create 1 P).
+Example c1 : composition := composition_create 0 Protocol.P.
+Example c1b : composition := (PAR (PRC (worker_create 0 OK)) (PRC (worker_create 1 Protocol.P)), resource_create 1).
