examples/CADP_Glued.v
@@ -10,18 +10,18 @@ Definition do_acquire_inner (c:tm) (s:state) (r:resource)
   let t : tm := unfold (AcquireInnerDef, AcquireInnerBody) AcquireInnerBody in
   (* ACT READ_LOCKED *)
   match read_locked e with
-  | None => (PRC ERR
+  | None => (PRC (ERR,
                 (add_error (Build_error 40
-                  "do_acquire_inner, read_locked e failed" (Build_error_info None (None, None))) s),
+                  "do_acquire_inner, read_locked e failed" (Build_error_info None (None, None))) s)),
                 r)
   | Some e =>
     (* IF (VAR LOCKED) *)
     match (get_local_var_value LOCKED (get_state e)) with
-    | BOOL true => (* REC_CALL 2 *) (PRC (SEQ t c) (get_state e), get_resource e)
-    | BOOL false => (PRC c (get_state e), get_resource e)
-    | _ => (PRC ERR
+    | BOOL true => (* REC_CALL 2 *) (PRC ((SEQ t c), (get_state e)), get_resource e)
+    | BOOL false => (PRC (c, (get_state e)), get_resource e)
+    | _ => (PRC (ERR,
                 (add_error (Build_error 41
-                  "do_acquire_inner, var locked not bool" (Build_error_info None (None, None))) (get_state e)),
+                  "do_acquire_inner, var locked not bool" (Build_error_info None (None, None))) (get_state e))),
                 get_resource e)
     end
   end
@@ -34,40 +34,34 @@ Definition do_acquire (c:tm) (s:state) (r:resource)
   let e : env := (s, r) in
   (* ACT (WRITE_NEXT THE_PID NIL) *)
   match write_next THE_PID NIL e with
-  | None => (PRC ERR
+  | None => (PRC (ERR,
                 (add_error (Build_error 50
-                  "do_acquire, write_next THE_PID NIL failed" (Build_error_info None (None, None))) s),
+                  "do_acquire, write_next THE_PID NIL failed" (Build_error_info None (None, None))) s)),
                 r)
   | Some e =>
     (* ACT FETCH_AND_STORE *)
-    match fetch_and_store e with
-    | None => (PRC ERR
-                  (add_error (Build_error 51
-                    "do_acquire, fetch_and_store failed" (Build_error_info None (None, None))) (get_state e)),
-                  (get_resource e))
-    | Some e =>
-      (* IF (EQ (VAR PREDECESSOR) (VAL NIL)) *)
-      match (get_local_var_value PREDECESSOR (get_state e)) with
-      | NIL => (* OK *) (PRC c (get_state e), get_resource e)
-      | _ =>
-        (* ACT (WRITE_LOCKED THE_PID (BOOL true)) *)
-        match write_locked THE_PID (BOOL true) e with
-        | None => (PRC ERR
-                      (add_error (Build_error 52
-                        "do_acquire, write_locked THE_PID (BOOL true) failed" (Build_error_info None (None, None))) (get_state e)),
+    let e:env := fetch_and_store e in
+    (* IF (EQ (VAR PREDECESSOR) (VAL NIL)) *)
+    match (get_local_var_value PREDECESSOR (get_state e)) with
+    | NIL => (* OK *) (PRC (c, (get_state e)), get_resource e)
+    | _ =>
+      (* ACT (WRITE_LOCKED THE_PID (BOOL true)) *)
+      match write_locked THE_PID (BOOL true) e with
+      | None => (PRC (ERR,
+                    (add_error (Build_error 52
+                      "do_acquire, write_locked THE_PID (BOOL true) failed" (Build_error_info None (None, None))) (get_state e))),
+                (get_resource e))
+      | Some e =>
+        (* ACT (WRITE_NEXT PREDECESSOR (GET THE_PID)) *)
+        match write_next PREDECESSOR (GET THE_PID) e with
+        | None => (PRC (ERR,
+                      (add_error (Build_error 53
+                        "do_acquire, write_next PREDECESSOR (GET THE_PID) failed" (Build_error_info None (None, None))) (get_state e))),
                   (get_resource e))
         | Some e =>
-          (* ACT (WRITE_NEXT PREDECESSOR (GET THE_PID)) *)
-          match write_next PREDECESSOR (GET THE_PID) e with
-          | None => (PRC ERR
-                        (add_error (Build_error 53
-                          "do_acquire, write_next PREDECESSOR (GET THE_PID) failed" (Build_error_info None (None, None))) (get_state e)),
-                    (get_resource e))
-          | Some e =>
-            (PRC (SEQ (AcquireInnerLoop) c) (get_state e)
-            , get_resource e
-            )
-          end
+          (PRC (SEQ (AcquireInnerLoop) c, get_state e)
+          , get_resource e
+          )
         end
       end
     end
@@ -82,23 +76,23 @@ Definition do_release_inner (c:tm) (s:state) (r:resource)
   let t : tm := unfold (ReleaseInnerDef, ReleaseInnerBody) ReleaseInnerBody in
   (* ACT READ_NEXT *)
   match read_next e with
-  | None => (PRC ERR
+  | None => (PRC (ERR,
                 (add_error (Build_error 45
-                  "do_release_inner, read_next e failed" (Build_error_info None (None, None))) s),
+                  "do_release_inner, read_next e failed" (Build_error_info None (None, None))) s)),
                 r)
   | Some e =>
     (* IF (EQ (VAL NIL) (VAR NEXT)) *)
     match (get_local_var_value NEXT (get_state e)) with
-    | NIL => (* REC_CALL 1 *) (PRC (SEQ t c) (get_state e), get_resource e)
+    | NIL => (* REC_CALL 1 *) (PRC ((SEQ t c), (get_state e)), get_resource e)
     | _ =>
       (* ACT (WRITE_LOCKED NEXT (BOOL false)) *)
       match write_locked NEXT (BOOL false) e with
-      | None => (PRC ERR
+      | None => (PRC (ERR,
                     (add_error (Build_error 46
-                      "do_release_inner, write_locked NEXT (BOOL false) failed" (Build_error_info None (None, None))) (get_state e)),
+                      "do_release_inner, write_locked NEXT (BOOL false) failed" (Build_error_info None (None, None))) (get_state e))),
                     (get_resource e))
       | Some e =>
-        (PRC c (get_state e), get_resource e)
+        (PRC (c, (get_state e)), get_resource e)
       end
     end
   end
@@ -110,39 +104,33 @@ Definition do_release (c:tm) (s:state) (r:resource)
   let e : env := (s, r) in
   (* ACT READ_NEXT *)
   match read_next e with
-  | None => (PRC ERR
+  | None => (PRC (ERR,
                 (add_error (Build_error 60
-                  "do_release, read_next e failed" (Build_error_info None (None, None))) s),
+                  "do_release, read_next e failed" (Build_error_info None (None, None))) s)),
                 r)
   | Some e =>
     (* IF (EQ (VAL NIL) (VAR NEXT)) *)
     match (get_local_var_value NEXT (get_state e)) with
     | NIL =>
       (* ACT COMPARE_AND_SWAP *)
-      match compare_and_swap e with
-      | None => (PRC ERR
-                    (add_error (Build_error 61
-                      "do_acquire, compare_and_swap failed" (Build_error_info None (None, None))) (get_state e)),
-                    (get_resource e))
-      | Some e =>
-        (* IF (EQ FLS (VAR SWAP)) *)
-        match (get_local_var_value SWAP (get_state e)) with
-        | BOOL false =>
-          (PRC (SEQ (ReleaseInnerLoop) c) (get_state e)
-          , get_resource e)
-        | _ => (* OK *) (PRC c (get_state e), get_resource e)
-        end
+      let e:env := compare_and_swap e in
+      (* IF (EQ FLS (VAR SWAP)) *)
+      match (get_local_var_value SWAP (get_state e)) with
+      | BOOL false =>
+        (PRC ((SEQ (ReleaseInnerLoop) c), (get_state e))
+        , get_resource e)
+      | _ => (* OK *) (PRC (c, (get_state e)), get_resource e)
       end
 
     | _ =>
       (* ACT (WRITE_LOCKED NEXT (BOOL false)) *)
       match write_locked NEXT (BOOL false) e with
-      | None => (PRC ERR
+      | None => (PRC (ERR,
                     (add_error (Build_error 61
-                      "do_release, write_locked NEXT (BOOL false) failed" (Build_error_info None (None, None))) (get_state e)),
+                      "do_release, write_locked NEXT (BOOL false) failed" (Build_error_info None (None, None))) (get_state e))),
                     (get_resource e))
       | Some e =>
-        (PRC c (get_state e), get_resource e)
+        (PRC (c, (get_state e)), get_resource e)
       end
     end
   end
@@ -153,60 +141,27 @@ Definition do_main_loop (b:tm) (s:state) (r:resource)
   : composition
   :=
   (* REC_DEF 0 *)
-  (PRC (unfold (PMainLoopDef, b) b) s, r)
+  (PRC ((unfold (PMainLoopDef, b) b), s), r)
   .
 
 Inductive bigstep : composition -> option label -> composition -> Prop :=
-  (*  0 *)
-  | DO_MAIN_LOOP : forall b s r,
-    bigstep (PRC (REC_DEF PMainLoopDef b) s, r) 
-            None 
-            (do_main_loop b s r)
-
-  (*  1 *)
-  | DO_ACQUIRE : forall c s r,
-    bigstep (PRC (SEQ (Acquire) (c)) s, r)
-            None
-            (do_acquire c s r)
-
-  (*  2 *)
-  | DO_RELEASE : forall c s r,
-    bigstep (PRC (SEQ (Release) (c)) s, r)
-            None
-            (do_release c s r)
-
-  (*  3 *)
-  | DO_ACQUIRE_INNER : forall c s r,
-    bigstep (PRC (SEQ (AcquireInnerLoop) c) s, r)
-            None
-            (do_acquire_inner c s r)
-
-  (*  4 *)
-  | DO_RELEASE_INNER : forall c s r,
-    bigstep (PRC (SEQ (ReleaseInnerLoop) c) s, r)
-            None
-            (do_release_inner c s r)
-
-  (*  5 *)
-  | DO_SEQ_ACT_ENTER : forall y s r,
-    bigstep (PRC (SEQ (ACT ENTER) y) s, r) 
-            (Some (ENTER, (get_pid s))) 
-            (PRC y s, r)
-
-  (*  6 *)
-  | DO_SEQ_ACT_LEAVE : forall y s r,
-    bigstep (PRC (SEQ (ACT LEAVE) y) s, r) 
-            (Some (LEAVE, (get_pid s))) 
-            (PRC y s, r)
-
-  (*  7 *)
-  | DO_PAR_L : forall a l1 l2 r gr1 gr2,
-    bigstep (l1, gr1) a (l2, gr2) ->
-    bigstep (PAR l1 r, gr1) a (PAR l2 r, gr2)
-
-  (*  8 *)
-  | DO_PAR_R : forall a l r1 r2 gr1 gr2,
-    bigstep (r1, gr1) a (r2, gr2) ->
-    bigstep (PAR l r1, gr1) a (PAR l r2, gr2)
-
-  .
+| DO_MAIN_LOOP : forall b s r,
+  bigstep (PRC (REC_DEF PMainLoopDef b, s), r) None (do_main_loop b s r)
+| DO_ACQUIRE : forall c s r,
+  bigstep (PRC (SEQ Acquire c, s), r) None (do_acquire c s r)
+| DO_RELEASE : forall c s r,
+  bigstep (PRC (SEQ Release c, s), r) None (do_release c s r)
+| DO_ACQUIRE_INNER : forall c s r,
+  bigstep (PRC (SEQ AcquireInnerLoop c, s), r) None (do_acquire_inner c s r)
+| DO_RELEASE_INNER : forall c s r,
+  bigstep (PRC (SEQ (ReleaseInnerLoop) c, s), r) None (do_release_inner c s r)
+| DO_SEQ_ACT_ENTER : forall y s r,
+  bigstep (PRC (SEQ (ACT ENTER) y, s), r) (Some (ENTER, (get_pid s))) (PRC (y, s), r)
+| DO_SEQ_ACT_LEAVE : forall y s r,
+  bigstep (PRC (SEQ (ACT LEAVE) y, s), r) (Some (LEAVE, (get_pid s))) (PRC (y, s), r)
+| DO_PAR_L : forall a l1 l2 r gr1 gr2,
+  bigstep (l1, gr1) a (l2, gr2) ->
+  bigstep (PAR l1 r, gr1) a (PAR l2 r, gr2)
+| DO_PAR_R : forall a l r1 r2 gr1 gr2,
+  bigstep (r1, gr1) a (r2, gr2) ->
+  bigstep (PAR l r1, gr1) a (PAR l r2, gr2).
